Revert non whyml-related changes

byteback-analysis/src/main/java/byteback/analysis/transformer/ExceptionInvariantTransformer.java
@@ -4,6 +4,7 @@ import byteback.analysis.Vimp;
 import byteback.analysis.vimp.VoidConstant;
 import byteback.util.Lazy;
 import java.util.HashSet;
+import java.util.List;
 import java.util.Map;
 import java.util.Set;
 import soot.Body;
@@ -19,68 +20,68 @@ import soot.util.Chain;
 
 public class ExceptionInvariantTransformer extends BodyTransformer {
 
-    private static final Lazy<ExceptionInvariantTransformer> instance = Lazy.from(ExceptionInvariantTransformer::new);
+	private static final Lazy<ExceptionInvariantTransformer> instance = Lazy.from(ExceptionInvariantTransformer::new);
 
-    private ExceptionInvariantTransformer() {
-    }
+	public static ExceptionInvariantTransformer v() {
+		return instance.get();
+	}
 
-    public static ExceptionInvariantTransformer v() {
-        return instance.get();
-    }
+	private ExceptionInvariantTransformer() {
+	}
 
-    @Override
-    public void internalTransform(final Body body, final String phaseName, final Map<String, String> options) {
-        if (body instanceof GrimpBody) {
-            transformBody(body);
-        } else {
-            throw new IllegalArgumentException("Can only transform Grimp");
-        }
-    }
+	@Override
+	public void internalTransform(final Body body, final String phaseName, final Map<String, String> options) {
+		if (body instanceof GrimpBody) {
+			transformBody(body);
+		} else {
+			throw new IllegalArgumentException("Can only transform Grimp");
+		}
+	}
 
-    public void transformBody(final Body body) {
-        final Chain<Unit> units = body.getUnits();
-        final LoopFinder loopFinder = new LoopFinder();
-        final Set<Loop> loops = loopFinder.getLoops(body);
-        final Set<Unit> trapHandlers = new HashSet<>();
+	public void transformBody(final Body body) {
+		final Chain<Unit> units = body.getUnits();
+		final LoopFinder loopFinder = new LoopFinder();
+		final Set<Loop> loops = loopFinder.getLoops(body);
+		final Set<Unit> trapHandlers = new HashSet<>();
 
-        for (final Trap trap : body.getTraps()) {
-            trapHandlers.add(trap.getHandlerUnit());
-        }
+		for (final Trap trap : body.getTraps()) {
+			trapHandlers.add(trap.getHandlerUnit());
+		}
 
-        for (final Loop loop : loops) {
-            if (loop.getHead() != loop.getBackJumpStmt()) {
-                final Value assertionValue = Vimp.v().newEqExpr(Vimp.v().newCaughtExceptionRef(), VoidConstant.v());
-                final Unit headUnit = loop.getHead();
-                final Unit newHeadUnit = Vimp.v().newAssertionStmt(assertionValue);
-                final Unit backJumpUnit = loop.getBackJumpStmt();
-                final Unit newBackJumpUnit = Vimp.v().newAssertionStmt(assertionValue);
-                final Set<Unit> annotatedUnits = new HashSet<>();
+		for (final Loop loop : loops) {
+			if (loop.getHead() != loop.getBackJumpStmt()) {
+				final Value assertionValue = Vimp.v().newEqExpr(Vimp.v().newCaughtExceptionRef(), VoidConstant.v());
+				final Unit headUnit = loop.getHead();
+				final Unit newHeadUnit = Vimp.v().newAssertionStmt(assertionValue);
+				final Unit backJumpUnit = loop.getBackJumpStmt();
+				final Unit newBackJumpUnit = Vimp.v().newAssertionStmt(assertionValue);
+				final Set<Unit> annotatedUnits= new HashSet<>();
 
-                units.insertBefore(newHeadUnit, headUnit);
-                headUnit.redirectJumpsToThisTo(newHeadUnit);
+				units.insertBefore(newHeadUnit, headUnit);
+				headUnit.redirectJumpsToThisTo(newHeadUnit);
 
-                units.insertBefore(newBackJumpUnit, backJumpUnit);
-                backJumpUnit.redirectJumpsToThisTo(newBackJumpUnit);
+				units.insertBefore(newBackJumpUnit, backJumpUnit);
+				backJumpUnit.redirectJumpsToThisTo(newBackJumpUnit);
 
-                for (final Unit exit : loop.getLoopExits()) {
-                    if (!annotatedUnits.contains(exit)) {
-                        final Unit newExitUnit = Vimp.v().newAssertionStmt(assertionValue);
-                        units.insertBefore(newExitUnit, exit);
-                        exit.redirectJumpsToThisTo(newExitUnit);
-                        annotatedUnits.add(exit);
+				for (final Unit exit : loop.getLoopExits()) {
+					if (!annotatedUnits.contains(exit)) {
+						final Unit newExitUnit = Vimp.v().newAssertionStmt(assertionValue);
+						units.insertBefore(newExitUnit, exit);
+						exit.redirectJumpsToThisTo(newExitUnit);
+						annotatedUnits.add(exit);
 
-                        for (final Unit exitTarget : loop.targetsOfLoopExit((Stmt) exit)) {
-                            if (!trapHandlers.contains(exitTarget) && !annotatedUnits.contains(exitTarget)) {
-                                final Unit newTargetUnit = Vimp.v().newAssertionStmt(assertionValue);
-                                units.insertBefore(newTargetUnit, exitTarget);
-                                exitTarget.redirectJumpsToThisTo(newTargetUnit);
-                                annotatedUnits.add(exitTarget);
-                            }
-                        }
-                    }
-                }
-            }
-        }
-    }
+						for (final Unit exitTarget : loop.targetsOfLoopExit((Stmt) exit)) {
+							if (!trapHandlers.contains(exitTarget) && !annotatedUnits.contains(exitTarget)) {
+								final Unit newTargetUnit = Vimp.v().newAssertionStmt(assertionValue);
+								units.insertBefore(newTargetUnit, exitTarget);
+								exitTarget.redirectJumpsToThisTo(newTargetUnit);
+								annotatedUnits.add(exitTarget);
+							}
+						}
+					}
+				}
+			}
+		}
+	}
 
 }
