example/GCD.bpl
@@ -1,4 +1,4 @@
-kind Reference;
+type Reference;
 
 const unique ~null : Reference;
 
@@ -6,9 +6,9 @@ const unique ~void : Reference;
 
 function ~isvoid(r : Reference) returns (bool) { (r == ~void) }
 
-kind Field a;
+type Field a;
 
-kind Store  = [Reference]<a>[Field (a)]a;
+type Store  = [Reference]<a>[Field (a)]a;
 
 function {:inline } ~heap.read<a>(h : Store, r : Reference, f : Field (a)) returns (a) { h[r][f] }
 
@@ -36,7 +36,7 @@ procedure ~new(t : Type) returns (~ret : Reference, ~exc : Reference);
   ensures ~allocated(~heap, ~ret);
   ensures (~exc == ~void);
 
-kind Type;
+type Type;
 
 const unique ~Object.Type : Field (Type);
 
@@ -48,13 +48,13 @@ function ~instanceof(h : Store, r : Reference, t : Type) returns (bool) { (~heap
 
 axiom (forall h : Store, t : Type :: !~instanceof(h, ~void, t));
 
-function ~kind.access(Type) returns (Reference);
+function ~type.reference(Type) returns (Reference);
 
-function ~kind.reference_inverse(Reference) returns (Type);
+function ~type.reference_inverse(Reference) returns (Type);
 
-axiom (forall t : Type :: {~kind.access(t)} (~kind.reference_inverse(~kind.access(t)) == t));
+axiom (forall t : Type :: {~type.reference(t)} (~type.reference_inverse(~type.reference(t)) == t));
 
-kind Box;
+type Box;
 
 function ~box<a>(a) returns (Box);
 
@@ -74,11 +74,11 @@ axiom (forall r : Reference :: (~lengthof(r) >= 0));
 
 axiom (forall h1 : Store, h2 : Store, r : Reference, i : int :: ((~heap.succ(h1, h2) && ((0 <= i) && (i < ~lengthof(r)))) ==> (~heap.read(h1, r, ~element(i)) == ~heap.read(h2, r, ~element(i)))));
 
-function ~array.kind(Type) returns (Type);
+function ~array.type(Type) returns (Type);
 
 function ~array.type_inverse(Type) returns (Type);
 
-axiom (forall t : Type :: {~array.kind(t)} (~array.type_inverse(~array.kind(t)) == t));
+axiom (forall t : Type :: {~array.type(t)} (~array.type_inverse(~array.type(t)) == t));
 
 function {:inline } ~array.read<b>(h : Store, a : Reference, i : int) returns (b) { (~unbox(~heap.read(h, a, ~element(i))) : b) }
 
@@ -86,7 +86,7 @@ function {:inline } ~array.update<b>(h : Store, a : Reference, i : int, v : b) r
 
 procedure ~array(t : Type, l : int) returns (~ret : Reference, ~exc : Reference);
   ensures (~ret != ~null);
-  ensures (~typeof(~heap, ~ret) == ~array.kind(t));
+  ensures (~typeof(~heap, ~ret) == ~array.type(t));
   ensures ~allocated(~heap, ~ret);
   ensures ((~lengthof(~ret) == l) && (~lengthof(~ret) >= 0));
   ensures (~exc == ~void);
@@ -156,47 +156,13 @@ function ~int_to_real(a : int) returns (real) { real(a) }
 
 function ~real_to_int(a : real) returns (int) { int(a) }
 
-const unique $java.lang.constant.Constable : Type;
-
-axiom ($java.lang.constant.Constable <: $java.lang.Object);
-
 const unique $java.lang.constant.ConstantDesc : Type;
 
 axiom ($java.lang.constant.ConstantDesc <: $java.lang.Object);
 
-const unique $java.io.Serializable : Type;
+const unique $java.lang.Appendable : Type;
 
-axiom ($java.io.Serializable <: $java.lang.Object);
-
-const unique $java.lang.CharSequence : Type;
-
-axiom ($java.lang.CharSequence <: $java.lang.Object);
-
-const unique $java.lang.Throwable : Type;
-
-axiom ($java.lang.Throwable <: $java.lang.Object);
-
-axiom ($java.lang.Throwable <: $java.io.Serializable);
-
-const unique $java.lang.Object : Type;
-
-axiom (forall t1 : Type, t2 : Type :: {(t1 <: $java.lang.String), (t2 <: $java.lang.Throwable)} (((t1 <: $java.lang.String) && (t2 <: $java.lang.Throwable)) ==> (!(t1 <: t2) && !(t2 <: t1))));
-
-axiom (forall t1 : Type, t2 : Type :: {(t1 <: $java.lang.String), (t2 <: $GCD)} (((t1 <: $java.lang.String) && (t2 <: $GCD)) ==> (!(t1 <: t2) && !(t2 <: t1))));
-
-axiom (forall t1 : Type, t2 : Type :: {(t1 <: $GCD), (t2 <: $java.lang.Throwable)} (((t1 <: $GCD) && (t2 <: $java.lang.Throwable)) ==> (!(t1 <: t2) && !(t2 <: t1))));
-
-const unique $java.lang.IllegalArgumentException : Type;
-
-axiom ($java.lang.IllegalArgumentException <: $java.lang.RuntimeException);
-
-const unique $java.lang.Comparable : Type;
-
-axiom ($java.lang.Comparable <: $java.lang.Object);
-
-const unique $java.lang.RuntimeException : Type;
-
-axiom ($java.lang.RuntimeException <: $java.lang.Exception);
+axiom ($java.lang.Appendable <: $java.lang.Object);
 
 const unique $java.lang.String : Type;
 
@@ -212,13 +178,113 @@ axiom ($java.lang.String <: $java.lang.constant.Constable);
 
 axiom ($java.lang.String <: $java.lang.constant.ConstantDesc);
 
-const unique $java.lang.Exception : Type;
+const unique $java.io.FilterOutputStream : Type;
 
-axiom ($java.lang.Exception <: $java.lang.Throwable);
+axiom ($java.io.FilterOutputStream <: $java.io.OutputStream);
+
+const unique $java.lang.CharSequence : Type;
+
+axiom ($java.lang.CharSequence <: $java.lang.Object);
+
+const unique $java.lang.Throwable : Type;
+
+axiom ($java.lang.Throwable <: $java.lang.Object);
+
+axiom ($java.lang.Throwable <: $java.io.Serializable);
+
+const unique $java.lang.Comparable : Type;
+
+axiom ($java.lang.Comparable <: $java.lang.Object);
 
 const unique $GCD : Type;
 
 axiom ($GCD <: $java.lang.Object);
+
+const unique $java.io.Flushable : Type;
+
+axiom ($java.io.Flushable <: $java.lang.Object);
+
+const unique $java.lang.Exception : Type;
+
+axiom ($java.lang.Exception <: $java.lang.Throwable);
+
+const unique $java.io.Closeable : Type;
+
+axiom ($java.io.Closeable <: $java.lang.Object);
+
+axiom ($java.io.Closeable <: $java.lang.AutoCloseable);
+
+const unique $java.lang.constant.Constable : Type;
+
+axiom ($java.lang.constant.Constable <: $java.lang.Object);
+
+const unique $java.lang.System : Type;
+
+axiom ($java.lang.System <: $java.lang.Object);
+
+const unique $java.io.PrintStream : Type;
+
+axiom ($java.io.PrintStream <: $java.io.FilterOutputStream);
+
+axiom ($java.io.PrintStream <: $java.lang.Appendable);
+
+axiom ($java.io.PrintStream <: $java.io.Closeable);
+
+const unique $java.io.Serializable : Type;
+
+axiom ($java.io.Serializable <: $java.lang.Object);
+
+const unique $java.io.OutputStream : Type;
+
+axiom ($java.io.OutputStream <: $java.lang.Object);
+
+axiom ($java.io.OutputStream <: $java.io.Closeable);
+
+axiom ($java.io.OutputStream <: $java.io.Flushable);
+
+const unique $java.lang.AutoCloseable : Type;
+
+axiom ($java.lang.AutoCloseable <: $java.lang.Object);
+
+const unique $java.lang.IllegalArgumentException : Type;
+
+axiom ($java.lang.IllegalArgumentException <: $java.lang.RuntimeException);
+
+const unique $java.lang.Object : Type;
+
+axiom (forall t1 : Type, t2 : Type :: {(t1 <: $java.io.OutputStream), (t2 <: $java.lang.System)} (((t1 <: $java.io.OutputStream) && (t2 <: $java.lang.System)) ==> (!(t1 <: t2) && !(t2 <: t1))));
+
+axiom (forall t1 : Type, t2 : Type :: {(t1 <: $java.lang.Throwable), (t2 <: $java.lang.String)} (((t1 <: $java.lang.Throwable) && (t2 <: $java.lang.String)) ==> (!(t1 <: t2) && !(t2 <: t1))));
+
+axiom (forall t1 : Type, t2 : Type :: {(t1 <: $java.lang.System), (t2 <: $java.lang.String)} (((t1 <: $java.lang.System) && (t2 <: $java.lang.String)) ==> (!(t1 <: t2) && !(t2 <: t1))));
+
+axiom (forall t1 : Type, t2 : Type :: {(t1 <: $java.io.OutputStream), (t2 <: $GCD)} (((t1 <: $java.io.OutputStream) && (t2 <: $GCD)) ==> (!(t1 <: t2) && !(t2 <: t1))));
+
+axiom (forall t1 : Type, t2 : Type :: {(t1 <: $GCD), (t2 <: $java.lang.String)} (((t1 <: $GCD) && (t2 <: $java.lang.String)) ==> (!(t1 <: t2) && !(t2 <: t1))));
+
+axiom (forall t1 : Type, t2 : Type :: {(t1 <: $java.io.OutputStream), (t2 <: $java.lang.String)} (((t1 <: $java.io.OutputStream) && (t2 <: $java.lang.String)) ==> (!(t1 <: t2) && !(t2 <: t1))));
+
+axiom (forall t1 : Type, t2 : Type :: {(t1 <: $java.lang.System), (t2 <: $GCD)} (((t1 <: $java.lang.System) && (t2 <: $GCD)) ==> (!(t1 <: t2) && !(t2 <: t1))));
+
+axiom (forall t1 : Type, t2 : Type :: {(t1 <: $GCD), (t2 <: $java.lang.Throwable)} (((t1 <: $GCD) && (t2 <: $java.lang.Throwable)) ==> (!(t1 <: t2) && !(t2 <: t1))));
+
+axiom (forall t1 : Type, t2 : Type :: {(t1 <: $java.lang.System), (t2 <: $java.lang.Throwable)} (((t1 <: $java.lang.System) && (t2 <: $java.lang.Throwable)) ==> (!(t1 <: t2) && !(t2 <: t1))));
+
+axiom (forall t1 : Type, t2 : Type :: {(t1 <: $java.io.OutputStream), (t2 <: $java.lang.Throwable)} (((t1 <: $java.io.OutputStream) && (t2 <: $java.lang.Throwable)) ==> (!(t1 <: t2) && !(t2 <: t1))));
+
+const unique $java.lang.RuntimeException : Type;
+
+axiom ($java.lang.RuntimeException <: $java.lang.Exception);
+
+const unique $java.lang.System.out : Field (Reference);
+
+function GCD.arguments_are_negative#boolean#short#short##(~heap : Store, _l0 : int, _l1 : int) returns (bool) { (~int.lte(_l0, 0) || ~int.lte(_l1, 0)) }
+
+function GCD.arguments_are_positive#boolean#short#short##(~heap : Store, _l0 : int, _l1 : int) returns (bool) { (~int.lte(_l0, 0) && ~int.lte(_l1, 0)) }
+
+procedure java.io.PrintStream.println#void#java.lang.String##(?this : Reference where ~instanceof(~heap, ?this, $java.io.PrintStream), ?p0 : Reference where ~instanceof(~heap, ?p0, $java.lang.String)) returns (~exc : Reference);
+  free ensures ~heap.succ(old(~heap), ~heap);
+  modifies ~heap;
 
 procedure GCD.$init$#void##(?l0 : Reference where ~instanceof(~heap, ?l0, $GCD)) returns (~exc : Reference)
   free ensures ~heap.succ(old(~heap), ~heap);
@@ -236,22 +302,22 @@ label1:
   return;
 }
 
-procedure java.lang.IllegalArgumentException.$init$#void#java.lang.String##(?this : Reference where ~instanceof(~heap, ?this, $java.lang.IllegalArgumentException), ?p0 : Reference where ~instanceof(~heap, ?p0, $java.lang.String)) returns (~exc : Reference);
-  ensures (true ==> (~exc == ~void));
+procedure java.lang.String.length#int##(?this : Reference where ~instanceof(~heap, ?this, $java.lang.String)) returns (~ret : int, ~exc : Reference);
   free ensures ~heap.succ(old(~heap), ~heap);
   modifies ~heap;
 
-procedure GCD.gcd#int#int#int##(?l0 : int, ?l1 : int) returns (~ret : int, ~exc : Reference)
-  ensures {:msg "GCD.java: (line 36): Error: The exceptional-precondition arguments_are_negative might not hold."}(old((~int.lte(?l0, 0) || ~int.lte(?l1, 0))) ==> ~instanceof(~heap, ~exc, $java.lang.IllegalArgumentException));
-  ensures {:msg "GCD.java: (line 36): Error: The postcondition result_is_gcd might not hold."}~implies(~not(GCD.arguments_are_negative#boolean#int#int##(~heap, ?l0, ?l1)), ~eq(~ret, GCD.gcd_recursive#int#int#int##(~heap, ?l0, ?l1)));
+procedure GCD.gcd#short#short#short##(?l0 : int, ?l1 : int) returns (~ret : int, ~exc : Reference)
+  ensures {:msg "GCD.java: (line 58): Error: The exceptional-precondition arguments_are_negative might not hold."}(old((~int.lte(?l0, 0) || ~int.lte(?l1, 0))) ==> ~instanceof(~heap, ~exc, $java.lang.IllegalArgumentException));
+  ensures {:msg "GCD.java: (line 58): Error: The postcondition result_is_gcd might not hold."}~implies(~not(GCD.arguments_are_negative#boolean#short#short##(~heap, ?l0, ?l1)), ~eq(~ret, GCD.gcd_recursive#short#short#short##(~heap, ?l0, ?l1)));
   free ensures ~heap.succ(old(~heap), ~heap);
   modifies ~heap;
 {
   var _l0 : int;
   var _l1 : int;
-  var _$stack4 : Reference where ~instanceof(~heap, _$stack4, $java.lang.IllegalArgumentException);
+  var _$stack7 : int;
   var _l2 : int;
   var _l3 : int;
+  var _$u0 : Reference where ~instanceof(~heap, _$u0, $java.lang.IllegalArgumentException);
   ~exc := ~void;
   _l0 := ?l0;
   _l1 := ?l1;
@@ -262,55 +328,74 @@ procedure GCD.gcd#int#int#int##(?l0 : int, ?l1 : int) returns (~ret : int, ~exc 
     goto label2;
   }
 label1:
-  call _$stack4, ~exc := ~new($java.lang.IllegalArgumentException);
-  call ~exc := java.lang.IllegalArgumentException.$init$#void#java.lang.String##(_$stack4, ~string.const(1364445960));
+  call _$u0, ~exc := ~new($java.lang.IllegalArgumentException);
+  call ~exc := java.lang.IllegalArgumentException.$init$#void#java.lang.String##(_$u0, ~string.const(1364445960));
   if ((~exc == ~void)) {
     goto label3;
   }
   return;
 label3:
-  ~exc := _$stack4;
+  ~exc := _$u0;
   return;
 label2:
+  call _$stack7, ~exc := java.lang.String.length#int##(~string.const(3053332));
+  if ((~exc == ~void)) {
+    goto label4;
+  }
+  return;
+label4:
+  if ((~cmp(_l0, _$stack7) <= 0)) {
+    goto label6;
+  }
+  call ~exc := java.io.PrintStream.println#void#java.lang.String##(~heap.read(~heap, ~type.reference($java.lang.System), $java.lang.System.out), ~string.const(2986048));
+  if ((~exc == ~void)) {
+    goto label6;
+  }
+  return;
+label6:
   _l2 := _l0;
   _l3 := _l1;
-label7:
-  assert {:msg "GCD.java: (line 45): Error: This assertion might not hold."}(~int.gt(_l2, 0) && ~int.gt(_l3, 0));
-  assert {:msg "GCD.java: (line 46): Error: This assertion might not hold."}~eq(GCD.gcd_recursive#int#int#int##(~heap, _l2, _l3), GCD.gcd_recursive#int#int#int##(~heap, _l0, _l1));
+label10:
+  assert {:msg "GCD.java: (line 75): Error: This assertion might not hold."}(~int.gt(_l2, 0) && ~int.gt(_l3, 0));
+  assert {:msg "GCD.java: (line 76): Error: This assertion might not hold."}~eq(GCD.gcd_recursive#short#short#short##(~heap, _l2, _l3), GCD.gcd_recursive#short#short#short##(~heap, _l0, _l1));
   assert (~exc == ~void);
   assert (~exc == ~void);
   if ((_l2 == _l3)) {
-    goto label4;
+    goto label7;
   }
   if ((_l2 <= _l3)) {
-    goto label5;
+    goto label8;
   }
   _l2 := (_l2 - _l3);
-  goto label7;
-label5:
+  goto label10;
+label8:
   _l3 := (_l3 - _l2);
   assert (~exc == ~void);
-  assert {:msg "GCD.java: (line 45): Error: This assertion might not hold."}(~int.gt(_l2, 0) && ~int.gt(_l3, 0));
-  assert {:msg "GCD.java: (line 46): Error: This assertion might not hold."}~eq(GCD.gcd_recursive#int#int#int##(~heap, _l2, _l3), GCD.gcd_recursive#int#int#int##(~heap, _l0, _l1));
-  goto label7;
-label4:
-  assert {:msg "GCD.java: (line 45): Error: This assertion might not hold."}(~int.gt(_l2, 0) && ~int.gt(_l3, 0));
-  assert {:msg "GCD.java: (line 46): Error: This assertion might not hold."}~eq(GCD.gcd_recursive#int#int#int##(~heap, _l2, _l3), GCD.gcd_recursive#int#int#int##(~heap, _l0, _l1));
+  assert {:msg "GCD.java: (line 75): Error: This assertion might not hold."}(~int.gt(_l2, 0) && ~int.gt(_l3, 0));
+  assert {:msg "GCD.java: (line 76): Error: This assertion might not hold."}~eq(GCD.gcd_recursive#short#short#short##(~heap, _l2, _l3), GCD.gcd_recursive#short#short#short##(~heap, _l0, _l1));
+  goto label10;
+label7:
+  assert {:msg "GCD.java: (line 75): Error: This assertion might not hold."}(~int.gt(_l2, 0) && ~int.gt(_l3, 0));
+  assert {:msg "GCD.java: (line 76): Error: This assertion might not hold."}~eq(GCD.gcd_recursive#short#short#short##(~heap, _l2, _l3), GCD.gcd_recursive#short#short#short##(~heap, _l0, _l1));
   assert (~exc == ~void);
   ~ret := _l2;
   return;
 }
-
-function GCD.gcd_recursive#int#int#int##(~heap : Store, _l0 : int, _l1 : int) returns (int) {
-if ~eq(_l0, _l1) then _l0
-else if ~int.gt(_l0, _l1) then GCD.gcd_recursive#int#int#int##(~heap, (_l0 - _l1), _l1)
-else GCD.gcd_recursive#int#int#int##(~heap, _l0, (_l1 - _l0)) }
 
 procedure java.lang.Object.$init$#void##(?this : Reference where ~instanceof(~heap, ?this, $java.lang.Object)) returns (~exc : Reference);
   ensures (true ==> (~exc == ~void));
   free ensures ~heap.succ(old(~heap), ~heap);
   modifies ~heap;
 
-function GCD.arguments_are_negative#boolean#int#int##(~heap : Store, _l0 : int, _l1 : int) returns (bool) { (~int.lte(_l0, 0) || ~int.lte(_l1, 0)) }
+procedure java.lang.IllegalArgumentException.$init$#void#java.lang.String##(?this : Reference where ~instanceof(~heap, ?this, $java.lang.IllegalArgumentException), ?p0 : Reference where ~instanceof(~heap, ?p0, $java.lang.String)) returns (~exc : Reference);
+  ensures (true ==> (~exc == ~void));
+  free ensures ~heap.succ(old(~heap), ~heap);
+  modifies ~heap;
 
-function GCD.arguments_are_positive#boolean#int#int##(~heap : Store, _l0 : int, _l1 : int) returns (bool) { (~int.lte(_l0, 0) && ~int.lte(_l1, 0)) }
+function GCD.gcd_recursive#short#short#short##(~heap : Store, _l0 : int, _l1 : int) returns (int) { if ~eq(_l0, _l1) then _l0 else if ~int.gt(_l0, _l1) then GCD.gcd_recursive2#short#short#short##(~heap, (_l0 - _l1), _l1) else GCD.gcd_recursive2#short#short#short##(~heap, _l0, (_l1 - _l0)) }
+
+function GCD.test#short#short##(~heap : Store, _l0 : int) returns (int) { if ~int.lte(_l0, 0) then 0 else GCD.test#short#short##(~heap, (_l0 - 1)) }
+
+function GCD.test2#boolean##(~heap : Store) returns (bool) { (forall _$stack1 : int :: ~int.lte(_$stack1, 0)) }
+
+function GCD.gcd_recursive2#short#short#short##(~heap : Store, _l0 : int, _l1 : int) returns (int) { if ~eq(_l0, _l1) then _l0 else if ~int.gt(_l0, _l1) then GCD.gcd_recursive#short#short#short##(~heap, (_l0 - _l1), _l1) else GCD.gcd_recursive#short#short#short##(~heap, _l0, (_l1 - _l0)) }
