byteback-frontend/boogie/src/test/resources/boogie/Simple.bpl
@@ -1,4 +1,4 @@
-kind Unit;
+type Unit;
 
 const unique unit : Unit;
 
